

**Part (a): Poisson's ratio**

$$\sigma_{ij} = \lambda \delta_{ij} \varepsilon_{kk} + 2\mu \varepsilon_{ij},$$

where  $\lambda$  and  $\mu$  are the Lamé parameters, and  $\varepsilon_{kk} = \varepsilon_{xx} + \varepsilon_{yy} + \varepsilon_{zz}$ .

Consider a uniaxial stress state,

$$\sigma_{xx} = \sigma, \quad \sigma_{yy} = \sigma_{zz} = 0.$$

Due to symmetry of loading,

$$\varepsilon_{yy} = \varepsilon_{zz} = \varepsilon_t.$$

Apply Hooke's law to the  $xx$ -component:

$$\sigma = \lambda(\varepsilon_{xx} + 2\varepsilon_t) + 2\mu \varepsilon_{xx}.$$

Apply Hooke's law to the  $yy$ -component where stress is zero:

$$0 = \lambda(\varepsilon_{xx} + 2\varepsilon_t) + 2\mu \varepsilon_t.$$

Solve the second equation for  $\varepsilon_{zz} = \varepsilon_{yy}$ :

$$\lambda \varepsilon_{xx} + 2(\lambda + \mu) \varepsilon_{yy} = 0,$$

or

$$\begin{aligned} \lambda \varepsilon_{xx} + 2(\lambda + \mu) \varepsilon_{zz} &= 0, \\ \varepsilon_{zz} = \varepsilon_{yy} &= -\frac{\lambda}{2(\lambda + \mu)} \varepsilon_{xx}. \end{aligned}$$

Poisson's ratio ( $\nu$ ) is defined as the negative ratio of lateral strain to longitudinal strain:

$$\nu = -\frac{\varepsilon_{yy}}{\varepsilon_{xx}} = -\frac{\varepsilon_{zz}}{\varepsilon_{xx}}.$$

Therefore,

$$\boxed{\nu = \frac{\lambda}{2(\lambda + \mu)}}.$$

**Part (b): Young's modulus**

$$0 = \lambda(\varepsilon_{xx} + 2\varepsilon_t) + 2\mu \varepsilon_t \quad \Rightarrow \quad \lambda \varepsilon_{xx} + (2\lambda + 2\mu) \varepsilon_t = 0,$$

so

$$\varepsilon_t = -\frac{\lambda}{2(\lambda + \mu)} \varepsilon_{xx}.$$

The  $xx$  component gives

$$\sigma = \lambda(\varepsilon_{xx} + 2\varepsilon_t) + 2\mu \varepsilon_{xx}.$$

Substitute  $\varepsilon_t$ :

$$\sigma = \lambda \varepsilon_{xx} + 2\lambda \varepsilon_t + 2\mu \varepsilon_{xx} = (\lambda + 2\mu) \varepsilon_{xx} + 2\lambda \left( -\frac{\lambda}{2(\lambda + \mu)} \varepsilon_{xx} \right).$$

Simplify:

$$\sigma = \left[ (\lambda + 2\mu) - \frac{\lambda^2}{\lambda + \mu} \right] \varepsilon_{xx} = \frac{(\lambda + 2\mu)(\lambda + \mu) - \lambda^2}{\lambda + \mu} \varepsilon_{xx}.$$

$$(\lambda + 2\mu)(\lambda + \mu) - \lambda^2 = \lambda^2 + 3\lambda\mu + 2\mu^2 - \lambda^2 = \mu(3\lambda + 2\mu).$$

Therefore

$$\sigma = \frac{\mu(3\lambda + 2\mu)}{\lambda + \mu} \varepsilon_{xx}.$$

By definition, Young's modulus is  $E = \frac{\sigma}{\varepsilon_{xx}}$  under uniaxial stress, so

$$\boxed{E = \frac{\mu(3\lambda + 2\mu)}{\lambda + \mu}}.$$